@prefix rdf: <http://www.w3.org/1999/02/22-rdf-syntax-ns#> .
@prefix Metarea: <http://metoffice.dataincubator.org/areas/> .
@prefix geo: <http://www.w3.org/2003/01/geo/wgs84_pos#> .
@prefix weather: <http://purl.org/ns/Meteo#> .
@prefix ns1: <http://metoffice.dataincubator.org/areas/os/> .
@prefix dct: <http://purl.org/dc/terms/> .
@prefix rdfs: <http://www.w3.org/2000/01/rdf-schema#> .
@prefix spatialrelations: <http://data.ordnancesurvey.co.uk/ontology/spatialrelations/> .
@prefix owl: <http://www.w3.org/2002/07/owl#> .
@prefix met: <http://metoffice.dataincubator.org/vocabs/metoffice/> .
@prefix ov: <http://open.vocab.org/terms/> .

<http://metoffice.dataincubator.org/vocabs/metoffice/>
    dct:creator <http://keithalexander.co.uk/id/me> ;
    a owl:Ontology ;
    rdfs:label "Met Office Vocabulary" ;
    ov:defines 
                met:identifier ,   
                met:MetOfficeRegion, 
                met:MetOfficeObservationSite , 
                met:MetOfficeLocation ,
                met:nearestObservationSite 
                .

met:identifier
    a rdf:Property ;
    rdfs:comment "a key used to identify a region or location by the Met Office website"@en ;
    rdfs:label "identifer" ;
    rdfs:subPropertyOf dct:identifier ;
    rdfs:isDefinedBy met: .

met:MetOfficeLocation
    a rdfs:Class ;
    rdfs:comment "A geographical location as used by the Met Office for declaring the spatial extent of their forecasts; contained within a met:MetofficeRegion "@en ;
    rdfs:label "Met Office Location"@en ;
    rdfs:subClassOf geo:SpatialThing ;
    rdfs:isDefinedBy met: .

met:MetOfficeObservationSite
    a rdfs:Class ;
    rdfs:comment "A site where Met Office records weather observations."@en ;
    rdfs:isDefinedBy <http://metoffice.dataincubator.org/vocabs/metoffice/> ;
    rdfs:label "Met Office Observation Site"@en ;
    rdfs:subClassOf geo:SpatialThing ;
    rdfs:isDefinedBy met: 
.

met:MetOfficeRegion
    a rdfs:Class ;
    rdfs:comment "A geographical region as used by the Met Office for declaring the spatial extent of their forecasts"@en ;
    rdfs:isDefinedBy <http://metoffice.dataincubator.org/vocabs/metoffice/> ;
    rdfs:label "Met Office Region"@en ;
    rdfs:subClassOf geo:SpatialThing  ;
.

met:nearestObservationSite
    a rdf:Property ;
    rdfs:comment "The closest Met Office Observation site"@en ;
    rdfs:label "Nearest Observation Site"@en ;
    rdfs:domain rdfs:Resource ;
    rdfs:range met:MetOfficeObservationSite  ;
    rdfs:isDefinedBy met:
  .


