@prefix rdf: <http://www.w3.org/1999/02/22-rdf-syntax-ns#> .
@prefix Metarea: <http://metoffice.dataincubator.org/areas/> .
@prefix geo: <http://www.w3.org/2003/01/geo/wgs84_pos#> .
@prefix weather: <http://purl.org/ns/Meteo#> .
@prefix ns1: <http://metoffice.dataincubator.org/areas/os/> .
@prefix dct: <http://purl.org/dc/terms/> .
@prefix rdfs: <http://www.w3.org/2000/01/rdf-schema#> .
@prefix spatialrelations: <http://data.ordnancesurvey.co.uk/ontology/spatialrelations/> .
@prefix owl: <http://www.w3.org/2002/07/owl#> .
@prefix met: <http://metoffice.dataincubator.org/vocabs/metoffice/> .
@base <http://metoffice.dataincubator.org/vocabs/metoffice/> .

<> 
	a owl:Ontology ;
	dct:creator <http://keithalexander.co.uk/id/me> ;
	rdfs:label "Met Office Vocabulary" 
	.

<metOfficeRegion> 
	a rdfs:Class ;
	rdfs:isDefinedBy <> ;
	rdfs:subClassOf geo:SpatialThing  ;
	rdfs:label "Met Office Region"@en ;
	rdfs:comment "A geographical region as used by the Met Office for declaring the spatial extent of their forecasts"@en
	.

<metOfficeLocation> 
	a rdfs:Class ;
	rdfs:subClassOf geo:SpatialThing  ;
	rdfs:label "Met Office Location"@en ;
	rdfs:comment "A geographical location as used by the Met Office for declaring the spatial extent of their forecasts; contained within a met:metofficeRegion "@en
	.


<metOfficeObservationSite>	
	a rdfs:Class ;
	rdfs:isDefinedBy <> ;
	rdfs:subClassOf geo:SpatialThing  ;
	rdfs:label "Met Office Observation Site"@en ;
	rdfs:comment "A site where Met Office records weather observations."@en ;
	.

<identifier> 
	a rdf:Property ;
	rdfs:subPropertyOf dct:identifier ;
	rdfs:label "identifer" ;
	rdfs:comment "a key used to identify a region or location by the Met Office website"@en 
	.
<nearestObservationSite>
	a rdf:Property ;
	rdfs:label "Nearest Observation Site"@en ;
	rdfs:comment "a key used to identify a region or location by the Met Office website"@en 
.